x86/ConstpropOpproof.v
@@ -292,8 +292,10 @@ Lemma addr_strength_reduction_correct:
   exists res', eval_addressing ge (Vptr sp Ptrofs.zero) addr' e##args' = Some res' /\ Val.lessdef res res'.
 Proof.
   unfold eval_addressing, addr_strength_reduction. destruct Archi.ptr64.
+- intros until res. destruct (addressing_valid (fst (addr_strength_reduction_64 addr args vl))).
   apply addr_strength_reduction_64_correct.
-  apply addr_strength_reduction_32_correct.
+  intros; exists res; auto.
+- apply addr_strength_reduction_32_correct.
 Qed.
 
 Lemma make_cmp_base_correct:
